backend/Debugvarproof.v
@@ -410,11 +410,11 @@ Inductive match_states: Linear.state ->  Linear.state -> Prop :=
       match_states (State s f sp c rs m)
                    (State ts tf sp tc rs m)
   | match_states_call:
-      forall s f rs m tf ts sz,
+      forall s f rs m tf ts sz tc,
       list_forall2 match_stackframes s ts ->
       transf_fundef f = OK tf ->
-      match_states (Callstate s f rs m sz)
-                   (Callstate ts tf rs m sz)
+      match_states (Callstate s f rs m sz tc)
+                   (Callstate ts tf rs m sz tc)
   | match_states_return:
       forall s rs m ts,
       list_forall2 match_stackframes s ts ->
@@ -534,14 +534,14 @@ Proof.
   apply plus_one.  econstructor. inv TRF; eauto. eauto.
   rewrite (parent_locset_match _ _ STACKS). constructor; auto.
 - (* internal function *)
-  monadInv H9. rename x into tf.
+  monadInv H10. rename x into tf.
   assert (MF: match_function f tf) by (apply transf_function_match; auto).
   inversion MF; subst.
   econstructor; split.
   apply plus_one. econstructor. eauto. eauto. reflexivity.
   constructor; auto.
 - (* external function *)
-  monadInv H9. econstructor; split.
+  monadInv H10. econstructor; split.
   apply plus_one. econstructor; eauto.
   eapply external_call_symbols_preserved; eauto. apply senv_preserved.
   constructor; auto.
@@ -560,7 +560,7 @@ Lemma transf_initial_states:
 Proof.
   intros. inversion H.
   exploit function_ptr_translated; eauto. intros [tf [A B]].
-  exists (Callstate nil tf (Locmap.init Vundef) m2 (fn_stack_requirements (prog_main tprog))); split.
+  exists (Callstate nil tf (Locmap.init Vundef) m2 (fn_stack_requirements (prog_main tprog)) false); split.
   econstructor; eauto. eapply (Genv.init_mem_transf_partial TRANSF); eauto.
   rewrite (match_program_main TRANSF), symbols_preserved. auto.
   rewrite <- H3. apply sig_preserved. auto.
