cfrontend/Csem.v
@@ -608,7 +608,7 @@ Inductive estep: state -> trace -> state -> Prop :=
       callred a m fd vargs ty i ->
       context RV RV C ->
       estep (ExprState f (C a) k e m)
-         E0 (Callstate fd vargs (Kcall f e C ty k) (Mem.push_new_stage m) (fn_stack_requirements i))
+         E0 (Callstate fd vargs (Kcall f e C ty k) m (fn_stack_requirements i))
 
   | step_stuck: forall C f a k e m K,
       context K RV C -> ~(imm_safe e K a m) ->
@@ -759,7 +759,7 @@ Inductive sstep: state -> trace -> state -> Prop :=
       alloc_variables empty_env m (f.(fn_params) ++ f.(fn_vars)) e m1 ->
       frame_adt_blocks fa = blocks_with_info e ->
       frame_adt_size fa = Z.max 0 sz ->
-      Mem.record_stack_blocks m1 fa = Some m1' ->
+      Mem.record_stack_blocks (Mem.push_new_stage m1) fa = Some m1' ->
       bind_parameters e m1' f.(fn_params) vargs m2 ->
       sstep (Callstate (Internal f) vargs k m sz)
          E0 (State f f.(fn_body) k e m2)
@@ -794,7 +794,7 @@ Inductive initial_state (p: program): state -> Prop :=
       type_of_fundef f = Tfunction Tnil type_int32s cc_default ->
       Mem.alloc m0 0 0 = (m1,b1) ->
       Mem.record_stack_blocks (Mem.push_new_stage m1) (make_singleton_frame_adt b1 0 0) = Some m2 ->
-      initial_state p (Callstate f nil Kstop (Mem.push_new_stage m2) (fn_stack_requirements (prog_main p))).
+      initial_state p (Callstate f nil Kstop m2 (fn_stack_requirements (prog_main p))).
 
 (** A final state is a [Returnstate] with an empty continuation. *)
 
