cfrontend/Csharpminor.v
@@ -397,7 +397,7 @@ Inductive step: state -> trace -> state -> Prop :=
       Genv.find_funct ge vf = Some fd ->
       funsig fd = sig ->
       step (State f (Scall optid sig a bl) k e le m)
-        E0 (Callstate fd vargs (Kcall optid f e le k) (Mem.push_new_stage m) (fn_stack_requirements id))
+        E0 (Callstate fd vargs (Kcall optid f e le k) m (fn_stack_requirements id))
 
   | step_builtin: forall f optid ef bl k e le m vargs t vres m',
       eval_exprlist e le m bl vargs ->
@@ -467,7 +467,7 @@ Inductive step: state -> trace -> state -> Prop :=
       alloc_variables empty_env m (fn_vars f) e m1 ->
       frame_adt_blocks fa = blocks_with_info e ->
       frame_adt_size fa = sz ->
-      Mem.record_stack_blocks m1 fa = Some m1' ->
+      Mem.record_stack_blocks (Mem.push_new_stage m1) fa = Some m1' ->
       bind_parameters f.(fn_params) vargs (create_undef_temps f.(fn_temps)) = Some le ->
       step (Callstate (Internal f) vargs k m sz)
         E0 (State f f.(fn_body) k e le m1')
@@ -497,7 +497,7 @@ Inductive initial_state (p: program): state -> Prop :=
       funsig f = signature_main ->
       Mem.alloc m0 0 0 = (m1,b1) ->
       Mem.record_stack_blocks (Mem.push_new_stage m1) (make_singleton_frame_adt b1 0 0) = Some m2 ->
-      initial_state p (Callstate f nil Kstop (Mem.push_new_stage m2) (fn_stack_requirements (prog_main p))).
+      initial_state p (Callstate f nil Kstop m2 (fn_stack_requirements (prog_main p))).
 
 (** A final state is a [Returnstate] with an empty continuation. *)
 
